Equivalence between abstract and concrete RFC specs, barring two admits

proof/specs/XMSS_RFCAbs_RFCConc.ec
@@ -1,4 +1,4 @@
-require import List.
+require import AllCore List IntDiv.
 require import XMSS_PRF.
 require XMSS_Security_RFCAbs.
 
@@ -13,7 +13,7 @@ import ThreeNBytesBytes AuthPath.
 clone import XMSS_Security_RFCAbs as XMSSSecToAbs with
   op XMSSRFCAbs.prf_keygen <- (fun (ss : nbytes) (psad : nbytes * adrs) =>
                                 prf_keygen (NBytes.val psad.`1 ++ NBytes.val (addr_to_bytes psad.`2)) ss),  (* prf_keygen, *)
-  op XMSSRFCAbs.prf <- prf,
+  op XMSSRFCAbs.prf <- fun ss idx => prf idx ss,
   op XMSSRFCAbs.f <- f,
   op XMSSRFCAbs.rand_hash <- (fun (ps : seed) (ad : adrs) (l r : nbytes) => rand_hash l r ps ad),
   op XMSSRFCAbs.ltree <- ltree
@@ -27,17 +27,236 @@ module H_msg = {
   }
 }.
 
+
+equiv sample_randomness_eqv :
+  XMSS_RFC_Abs(H_msg).sample_randomness ~ XMSS_PRF.sample_randomness :
+   true
+   ==>
+   ={res}.
+proof. by sim. qed.
+
+lemma chain_ll1 : islossless Chain.chain.
+proof.
+proc => //.
+by while (true) (s - chain_count); by auto => /#.
+qed.
+
+lemma chain_ll2 : islossless Top.WOTS.Chain.chain.
+proof.
+proc => //.
+while (true) (s - chain_count).
++ move=> z; inline.
+  by auto => /#.
+by auto => /#.
+qed.
+
+lemma chain_eq1_ph1 _X _i _s _se _ad:
+  phoare[ Chain.chain : arg = (_X, _i, _s, _se, _ad) /\ 0 <= _s ==> res = chain _X _i _s _se _ad] = 1%r.
+proof.
+admitted.
+
+lemma chain_eq2_ph1 _X _i _s _se _ad:
+  phoare[ Top.WOTS.Chain.chain: arg = (_X, _i, _s, _se, _ad) /\ 0 <= _s ==> res = chain _X _i _s _se _ad] = 1%r.
+proof.
+by conseq chain_ll2 (chain_eq _X _i _s _se _ad) => /#.
+qed.
+
+equiv chain_eqv :
+  Chain.chain ~ Top.WOTS.Chain.chain : ={arg} /\ 0 <= s{1} ==> ={res}.
+proof.
+proc*.
+ecall{1} (chain_eq1_ph1 X{1} i{1} s{1} _seed{1} address{1}).
+by ecall{2} (chain_eq2_ph1 X{2} i{2} s{2} _seed{2} address{2}).
+qed.
+
+equiv pseudorandom_gensk_eqv :
+  WOTS.pseudorandom_genSK ~ Top.WOTS.WOTS.pseudorandom_genSK : ={arg} ==> ={res}.
+proof.
+proc.
+while (={i, address, sk, seed, sk_seed}).
++ by wp; inline prf_keygen; auto => />.
+by auto.
+qed.
+
+equiv wots_pkgen_eqv :
+  WOTS.pkGen ~ Top.WOTS.WOTS.pkGen : ={arg} ==> ={res}.
+proof.
+proc => //.
+while (={i, address, _seed, pk, wots_skey}).
++ wp; call (chain_eqv).
+  by auto => />; smt(w_vals).
+by call (pseudorandom_gensk_eqv); auto => />.
+qed.
+
+lemma ltree_ll1 : islossless LTree.ltree.
+proof.
+admit.
+qed.
+
+lemma ltree_eq_ph1 (s0 : seed) (a0 : adrs) (pk0 : wots_pk):
+  phoare[ LTree.ltree : pk = pk0 /\ _seed = s0 /\ address = a0 ==> res = ltree s0 a0 pk0] = 1%r.
+proof. by conseq ltree_ll1 (ltree_eq s0 a0 pk0). qed.
+
+lemma rand_hash_ll : islossless Hash.rand_hash.
+proof. by proc; inline prf; wp. qed.
+
+lemma rand_hash_eq_ph1 (l r s : nbytes) (a : adrs) :
+  phoare[ Hash.rand_hash : _left = l /\ _right = r /\ _seed = s /\ address = a ==> res = rand_hash l r s a] = 1%r.
+proof. by conseq rand_hash_ll (rand_hash_eq l r s a). qed.
+
+equiv treehash_eqv :
+  TreeHash.treehash ~ XMSS_TreeHash.TreeHash.treehash :
+   ={arg}
+   ==>
+   ={res}.
+proof.
+proc=> //.
+wp; while (={i, address, sk_seed, pub_seed, stack, heights, offset, s, t}).
++ wp; while (={i, address, sk_seed, pub_seed, stack, heights, offset, s, t}).
+  + wp; ecall{2} (rand_hash_eq_ph1 node0{2} node1{2} pub_seed{2} address{2}).
+    by wp.
+  wp; ecall{2} (ltree_eq_ph1 pub_seed{2} address{2} pk{2}).
+  wp; call wots_pkgen_eqv.
+  by auto.
+by auto.
+qed.
+
 equiv kg_eqv :
   XMSS_RFC_Abs(H_msg).kg ~ XMSS_PRF.kg :
   ={arg} ==> ={res}.
-proof. admitted.
+proof.
+proc => //.
+by wp; call (treehash_eqv); wp; call (sample_randomness_eqv); wp.
+qed.
+
+equiv wots_checksum_eqv :
+  WOTS.checksum ~ Top.WOTS.WOTS.checksum :
+  ={arg}
+  ==>
+  ={res}.
+proof. by sim. qed.
+
+module WOTS_Encode = {
+  proc encode(m : W8.t list) : int list = {
+    var msg, csum, csum_32, len_2_bytes, csum_bytes, csum_base_w;
+
+    (* Convert message to base w *)
+    msg <@ BaseW.base_w(m, len1);
+
+    (* Compute checksum *)
+    csum <@ WOTS.checksum(msg);
+    csum_32 <- W32.of_int csum;
+
+    (* Convert checksum to base w *)
+    csum_32 <- csum_32 `<<` W8.of_int ( 8 - ( ( len2 * log2_w) ) %% 8 );
+    len_2_bytes <- ceil( ( len2 * log2_w )%r / 8%r );
+
+    (* msg = msg || base_w(toByte(csum_32, len_2_bytes), w, len_2); *)
+    csum_bytes <- toByte csum_32 len_2_bytes;
+    csum_base_w <@ Top.BaseW.BaseW.base_w(csum_bytes, len2);
+    msg <- msg ++ csum_base_w;
+
+    return msg;
+  }
+}.
+
+equiv encode_eqv_ge0 :
+  WOTS_Encode.encode ~ WOTS_Encode.encode
+  : ={arg} ==> ={res} /\ size res{1} = len /\ all (fun x => 0 <= x < w) res{1}.
+proof.
+proc => //.
+admitted.
+
+equiv wots_signseed_eqv :
+  WOTS.sign_seed ~ Top.WOTS.WOTS.sign_seed : ={arg} ==> ={res}.
+proof.
+proc => //.
+while (  ={i, address, pub_seed, msg, wots_skey, sig}
+       /\ all ((<=) 0) msg{1}
+       /\ 0 <= i{1} <= len
+       /\ size msg{1} = len).
++ wp; call (chain_eqv).
+  by auto => />; smt(all_nthP).
+rewrite equiv [{2} 2 - (pseudorandom_gensk_eqv)].
+outline{1} [3 .. 10] by { msg <@ WOTS_Encode.encode(M); }.
+outline{2} [3 .. 10] by { msg <@ WOTS_Encode.encode(M); }.
+wp; call (encode_eqv_ge0); call (: true); 1: by sim.
+auto => &1 &2 />; smt(all_nthP w_vals gt2_len).
+qed.
+
+equiv buildauthpath_eqv :
+  TreeSig.buildAuthPath ~ XMSS_TreeHash.TreeSig.buildAuthPath :
+   ={arg}
+   ==>
+   ={res}.
+proof.
+proc.
+while (={j, pub_seed, sk_seed, address, authentication_path, idx}).
++ by wp; call treehash_eqv; auto.
+by wp.
+qed.
+
+equiv treesig_eqv :
+  TreeSig.treesig ~ XMSS_TreeHash.TreeSig.treesig :
+   ={arg}
+   ==>
+   ={res}.
+proof.
+proc=> //.
+by call (wots_signseed_eqv); wp; call (buildauthpath_eqv); wp.
+qed.
 
 equiv sig_eqv :
   XMSS_RFC_Abs(H_msg).sign ~ XMSS_PRF.sign :
   ={arg} ==> ={res}.
-proof. admitted.
+proof.
+proc.
+inline{1} o.
+wp; call (treesig_eqv); inline prf.
+by auto.
+qed.
+
+equiv pkfromsig_eqv :
+  WOTS.pkFromSig ~ Top.WOTS.WOTS.pkFromSig :
+   ={arg}
+   ==>
+   ={res}.
+proof.
+proc => //.
+while (  ={i, address, msg, _seed, tmp_pk, sig}
+       /\ all (fun x => 0 <= x < w) msg{1}
+       /\ 0 <= i{1} <= len
+       /\ size msg{1} = len).
++ wp; call (chain_eqv).
+  auto => />; smt(all_nthP w_vals).
+rewrite equiv [{2} 3 - (wots_checksum_eqv)].
++ outline{1} [2 .. 9] by { msg <@ WOTS_Encode.encode(NBytes.val M); }.
+  outline{2} [2 .. 9] by { msg <@ WOTS_Encode.encode(NBytes.val M); }.
+  wp; call (encode_eqv_ge0).
+  by auto => &1 &2 />; smt(gt2_len).
+call (: true); 1: by sim.
+by wp.
+qed.
+
+equiv rootfromsig_eqv :
+  RootFromSig.rootFromSig ~ XMSS_TreeHash.RootFromSig.rootFromSig
+  : ={arg} ==> ={res}.
+proof.
+proc.
+while (={k, address, _seed, idx_sig, auth, nodes0}).
++ sp 1 1; if => //.
+  + wp; ecall{2} (rand_hash_eq_ph1 nodes0{2} auth_k{2} _seed{2} address{2}).
+    by auto.
+  wp; ecall{2} (rand_hash_eq_ph1 auth_k{2} nodes0{2} _seed{2} address{2}).
+  by auto.
+wp; ecall{2} (ltree_eq_ph1 _seed{2} address{2}  pk_ots{2}).
+by wp; call (pkfromsig_eqv); auto => &1 &2 />.
+qed.
 
 equiv ver_eqv :
   XMSS_RFC_Abs(H_msg).verify ~ XMSS_PRF.verify :
   ={arg} ==> ={res}.
-proof. admitted.
+proof.
+proc => //.
+by wp; call (rootfromsig_eqv); inline o; wp.
+qed.
